code/salsa-family/Hacl.Impl.Salsa20.fst
@@ -325,6 +325,8 @@ let lemma_u64_of_u32s (low:U32.t) (high:U32.t) : Lemma (low32_of_u64 (u64_of_u32
   Math.Lemmas.lemma_div_mod (UInt64.v (u64_of_u32s low high)) (pow2 32)
 
 
+#reset-options "--max_fuel 0  --z3rlimit 100"
+
 [@ "c_inline"]
 private
 val salsa20_core:
@@ -348,18 +350,18 @@ let salsa20_core log k st ctr =
   let h0 = ST.get() in
   let c0 = uint32_to_sint32 (low32_of_u64 ctr) in
   let c1 = uint32_to_sint32 (high32_of_u64 ctr) in
-  let h_1 = ST.get() in
+  let h1 = ST.get() in
   st.(8ul) <- c0;
   let h_ = ST.get() in
-  cut (as_seq h_ st == Seq.upd (as_seq h_1 st) 8 (c0));
+  cut (as_seq h_ st == Seq.upd (as_seq h1 st) 8 (c0));
   st.(9ul) <- c1;
-  let h_2 = ST.get() in
-  cut (as_seq h_2 st == Seq.upd (as_seq h_ st) 9 (c1));
-  cut (get h_2 st 8 == c0 /\ get h_2 st 9 == c1);
-  cut (let s = as_seq h0 st in let s' = as_seq h_2 st in s' == Seq.upd (Seq.upd s 8 c0) 9 c1);
+  let h2 = ST.get() in
+  cut (as_seq h2 st == Seq.upd (as_seq h_ st) 9 (c1));
+  cut (get h2 st 8 == c0 /\ get h2 st 9 == c1);
+  cut (let s = as_seq h0 st in let s' = as_seq h2 st in s' == Seq.upd (Seq.upd s 8 c0) 9 c1);
   lemma_invariant (reveal_h32s (as_seq h0 st)) (Ghost.reveal log).k (Ghost.reveal log).n (uint64_to_sint64 (u64_of_u32s (h32_to_u32 (get h0 st 8)) (h32_to_u32 (get h0 st 9)))) (uint64_to_sint64 ctr);
   lemma_u64_of_u32s (h32_to_u32 c0) (h32_to_u32 c1);
-  cut (invariant log h_2 st);
+  cut (invariant log h2 st);
   copy_state k st;
   rounds k;
   sum_states k st;
